

Section 3.2.4: Batch (Way A) and Sequential (Way B) Derivations

1 Problem Setup

We measure the same unknown scalar x repeatedly. For $i = 1, \dots, k$,

$$y_i = x + \nu_i, \quad \nu_i \sim \mathcal{N}(0, 1), \quad (1)$$

with $\{\nu_i\}$ independent. After k measurements, we will derive the estimate \hat{x}_k and its variance $\text{Var}(\hat{x}_k)$ in two ways:

- **Way A (Batch):** stack all measurements and solve once.
- **Way B (Sequential):** update (\hat{x}_k, P_k) recursively when a new measurement arrives.

2 Way A: Batch (All-at-Once) Derivation

2.1 Step 1: Stack measurements into a single linear system

Define

$$y \triangleq \begin{bmatrix} y_1 \\ \vdots \\ y_k \end{bmatrix} \in \mathbb{R}^{k \times 1}, \quad \nu \triangleq \begin{bmatrix} \nu_1 \\ \vdots \\ \nu_k \end{bmatrix} \in \mathbb{R}^{k \times 1}, \quad C \triangleq \begin{bmatrix} 1 \\ \vdots \\ 1 \end{bmatrix} \in \mathbb{R}^{k \times 1}. \quad (2)$$

Then all k scalar equations can be written compactly as

$$y = Cx + \nu. \quad (3)$$

Since each $\nu_i \sim \mathcal{N}(0, 1)$ and they are independent,

$$\nu \sim \mathcal{N}(0, I_k). \quad (4)$$

2.2 Step 2: Write the likelihood and the least-squares objective

Given x , the measurement vector y is Gaussian:

$$p(y \mid x) = \mathcal{N}(Cx, I_k). \quad (5)$$

Up to an additive constant independent of x , the negative log-likelihood is

$$-\log p(y \mid x) = \frac{1}{2}(y - Cx)^\top I_k^{-1}(y - Cx) = \frac{1}{2}\|y - Cx\|^2. \quad (6)$$

Thus maximizing likelihood is equivalent to minimizing the least-squares cost

$$J(x) \triangleq \|y - Cx\|^2. \quad (7)$$

2.3 Step 3: Solve the least-squares problem (normal equations)

Expand $J(x)$:

$$J(x) = (y - Cx)^\top (y - Cx) \quad (8)$$

$$= y^\top y - 2x C^\top y + x^2 C^\top C. \quad (9)$$

Differentiate with respect to the scalar x and set to zero:

$$\frac{dJ}{dx} = -2C^\top y + 2x C^\top C = 0 \implies \hat{x}_k = (C^\top C)^{-1} C^\top y. \quad (10)$$

Now plug in the special $C = \mathbf{1}_k$:

$$C^\top C = \mathbf{1}_k^\top \mathbf{1}_k = k, \quad C^\top y = \sum_{i=1}^k y_i. \quad (11)$$

Hence

$$\boxed{\hat{x}_k = \frac{1}{k} \sum_{i=1}^k y_i.} \quad (12)$$

2.4 Step 4: Derive the variance of the batch estimate

Start from

$$\hat{x}_k = (C^\top C)^{-1} C^\top y \quad (13)$$

$$= (C^\top C)^{-1} C^\top (Cx + \nu) \quad (14)$$

$$= x + (C^\top C)^{-1} C^\top \nu. \quad (15)$$

Therefore the estimation error is

$$\tilde{x}_k \triangleq \hat{x}_k - x = (C^\top C)^{-1} C^\top \nu. \quad (16)$$

Compute its variance:

$$\text{Var}(\hat{x}_k) = \text{Var}(\tilde{x}_k) \quad (17)$$

$$= (C^\top C)^{-1} C^\top \text{Cov}(\nu) C (C^\top C)^{-1}. \quad (18)$$

Since $\text{Cov}(\nu) = I_k$,

$$\text{Var}(\hat{x}_k) = (C^\top C)^{-1} C^\top I_k C (C^\top C)^{-1} = (C^\top C)^{-1}. \quad (19)$$

And because $C^\top C = k$,

$$\boxed{\text{Var}(\hat{x}_k) = \frac{1}{k}.} \quad (20)$$

3 Way B: Sequential (Recursive) Derivation

3.1 Step 0: Treat the first k measurements as a Gaussian prior

From Way A, after k unit-variance measurements,

$$\hat{x}_k = \frac{1}{k} \sum_{i=1}^k y_i, \quad P_k \triangleq \text{Var}(\hat{x}_k) = \frac{1}{k}. \quad (21)$$

Interpret this as a prior distribution for x conditioned on the first k measurements:

$$x \mid y_{1:k} \sim \mathcal{N}(\hat{x}_k, P_k). \quad (22)$$

Now obtain one more measurement

$$y_{k+1} = x + \nu_{k+1}, \quad \nu_{k+1} \sim \mathcal{N}(0, \sigma^2), \quad (23)$$

independent of everything else.

3.2 Step 1: Posterior is proportional to prior times likelihood

Prior:

$$p(x \mid y_{1:k}) \propto \exp\left(-\frac{1}{2P_k}(x - \hat{x}_k)^2\right). \quad (24)$$

Likelihood:

$$p(y_{k+1} \mid x) \propto \exp\left(-\frac{1}{2\sigma^2}(y_{k+1} - x)^2\right). \quad (25)$$

Multiply:

$$p(x \mid y_{1:k+1}) \propto \exp\left(-\frac{1}{2P_k}(x - \hat{x}_k)^2 - \frac{1}{2\sigma^2}(y_{k+1} - x)^2\right). \quad (26)$$

This exponent is quadratic in x , so the posterior is Gaussian.

3.3 Step 2: Expand and collect terms in x

Expand:

$$(x - \hat{x}_k)^2 = x^2 - 2\hat{x}_k x + \hat{x}_k^2, \quad (y_{k+1} - x)^2 = x^2 - 2y_{k+1}x + y_{k+1}^2. \quad (27)$$

Ignoring constants independent of x , the exponent becomes

$$-\frac{1}{2} \left[\left(\frac{1}{P_k} + \frac{1}{\sigma^2} \right) x^2 - 2 \left(\frac{\hat{x}_k}{P_k} + \frac{y_{k+1}}{\sigma^2} \right) x \right] + \text{const.} \quad (28)$$

Match this with the canonical Gaussian form

$$-\frac{1}{2} \left[\frac{1}{P_{k+1}} x^2 - 2 \frac{\hat{x}_{k+1}}{P_{k+1}} x \right] + \text{const.} \quad (29)$$

3.4 Step 3: Read off the variance update (information form)

Matching x^2 coefficients yields

$$\boxed{\frac{1}{P_{k+1}} = \frac{1}{P_k} + \frac{1}{\sigma^2}}. \quad (30)$$

Since $P_k = 1/k$, we have $1/P_k = k$, so

$$\frac{1}{P_{k+1}} = k + \frac{1}{\sigma^2} \implies \boxed{P_{k+1} = \frac{1}{k + \frac{1}{\sigma^2}} = \frac{\sigma^2}{\sigma^2 k + 1}}. \quad (31)$$

3.5 Step 4: Read off the mean update

Matching linear coefficients yields

$$\boxed{\frac{\hat{x}_{k+1}}{P_{k+1}} = \frac{\hat{x}_k}{P_k} + \frac{y_{k+1}}{\sigma^2}}. \quad (32)$$

Thus

$$\hat{x}_{k+1} = P_{k+1} \left(\frac{\hat{x}_k}{P_k} + \frac{y_{k+1}}{\sigma^2} \right). \quad (33)$$

Using $1/P_k = k$ and $P_{k+1} = \frac{1}{k+1/\sigma^2}$,

$$\hat{x}_{k+1} = \frac{1}{k + \frac{1}{\sigma^2}} \left(k\hat{x}_k + \frac{1}{\sigma^2}y_{k+1} \right). \quad (34)$$

This shows \hat{x}_{k+1} is a weighted average of \hat{x}_k and y_{k+1} , weighted by their precisions.

3.6 Step 5: Convert to innovation form

Subtract \hat{x}_k :

$$\hat{x}_{k+1} - \hat{x}_k = \frac{k\hat{x}_k + \frac{1}{\sigma^2}y_{k+1} - \hat{x}_k \left(k + \frac{1}{\sigma^2}\right)}{k + \frac{1}{\sigma^2}} \quad (35)$$

$$= \frac{\frac{1}{\sigma^2}(y_{k+1} - \hat{x}_k)}{k + \frac{1}{\sigma^2}} \quad (36)$$

$$= \frac{y_{k+1} - \hat{x}_k}{\sigma^2 k + 1}, \quad (37)$$

where the last step multiplies numerator and denominator by σ^2 . Therefore

$$\boxed{\hat{x}_{k+1} = \hat{x}_k + \frac{y_{k+1} - \hat{x}_k}{\sigma^2 k + 1}}. \quad (38)$$